code/chacha20/Hacl.Spec.Chacha20.Vec.fst
@@ -229,7 +229,7 @@ let chacha20_encrypt_last #w st0 incr len b =
 val chacha20_update:
     #w:lanes
   -> st0: state w
-  -> msg: bytes{length msg <= max_size_t}
+  -> msg: bytes{length msg / size_block <= max_size_t}
   -> cipher: bytes{length cipher == length msg}
 let chacha20_update #w st0 msg =
   let cipher = msg in
@@ -242,7 +242,7 @@ val chacha20_encrypt_bytes:
   -> k: key
   -> n: nonce
   -> c: counter
-  -> msg: bytes{length msg <= max_size_t}
+  -> msg: bytes{length msg / size_block <= max_size_t}
   -> cipher: bytes{length cipher == length msg}
 
 let chacha20_encrypt_bytes #w key nonce ctr0 msg =
@@ -254,7 +254,7 @@ val chacha20_decrypt_bytes:
   -> k: key
   -> n: nonce
   -> c: counter
-  -> cipher: bytes{length cipher <= max_size_t}
+  -> cipher: bytes{length cipher / size_block <= max_size_t}
   -> msg: bytes{length cipher == length msg}
 
 let chacha20_decrypt_bytes #w key nonce ctr0 cipher =
